Made all values pre-normalized

01Expression/Evaluate.thy
@@ -8,20 +8,17 @@ inductive evaluate :: "expr \<Rightarrow> expr \<Rightarrow> bool" (infix "\<lea
 | ev_app_let [simp]: "is_value e\<^sub>1\<^sub>2 \<Longrightarrow> App (Let e\<^sub>1\<^sub>1 e\<^sub>1\<^sub>2) e\<^sub>2 \<leadsto> Let e\<^sub>1\<^sub>1 (App e\<^sub>1\<^sub>2 (incr\<^sub>e\<^sub>e 0 e\<^sub>2))"
 | ev_let1 [simp]: "e\<^sub>2 \<leadsto> e\<^sub>2' \<Longrightarrow> Let e\<^sub>1 e\<^sub>2 \<leadsto> Let e\<^sub>1 e\<^sub>2'"
 | ev_let2 [simp]: "e\<^sub>1 \<leadsto> e\<^sub>1' \<Longrightarrow> head_var e\<^sub>2 = Some 0 \<Longrightarrow> Let e\<^sub>1 e\<^sub>2 \<leadsto> Let e\<^sub>1' e\<^sub>2"
-| ev_let3 [simp]: "is_value e\<^sub>1 \<Longrightarrow> head_var e\<^sub>2 = Some 0 \<Longrightarrow> Let e\<^sub>1 e\<^sub>2 \<leadsto> subst\<^sub>e\<^sub>e 0 e\<^sub>1 e\<^sub>2"
-| ev_rec [simp]: "list_all is_var vs \<Longrightarrow> \<not> is_var e \<Longrightarrow> 
-    Rec (vs @ [e] @ nvs) \<leadsto> Let e (Rec (map (incr\<^sub>e\<^sub>e 0) vs @ [Var 0] @ map (incr\<^sub>e\<^sub>e 0) nvs))" 
+| ev_let3 [simp]: "is_value e\<^sub>1 \<Longrightarrow> head_var e\<^sub>2 = Some 0 \<Longrightarrow> 
+    Let e\<^sub>1 e\<^sub>2 \<leadsto> Let e\<^sub>1 (subst\<^sub>e\<^sub>e 0 (incr\<^sub>e\<^sub>e 0 e\<^sub>1) e\<^sub>2)"
 | ev_proj1 [simp]: "e \<leadsto> e' \<Longrightarrow> Proj e l \<leadsto> Proj e' l"
-| ev_proj2 [simp]: "list_all is_var fs \<Longrightarrow> lookup l fs = Some e \<Longrightarrow> Proj (Rec fs) l \<leadsto> e" 
+| ev_proj2 [simp]: "lookup l fs = Some x \<Longrightarrow> Proj (Rec fs) l \<leadsto> Var x" 
 | ev_proj_let [simp]: "is_value e\<^sub>2 \<Longrightarrow> Proj (Let e\<^sub>1 e\<^sub>2) l \<leadsto> Let e\<^sub>1 (Proj e\<^sub>2 l)" 
-| ev_inj [simp]: "\<not> is_var e \<Longrightarrow> Inj l ts e \<leadsto> Let e (Inj l ts (Var 0))"
 | ev_case1 [simp]: "e \<leadsto> e' \<Longrightarrow> Case e t cs \<leadsto> Case e' t cs"
-| ev_case2 [simp]: "is_var e \<Longrightarrow> lookup l cs = Some e' \<Longrightarrow> Case (Inj l ts e) t cs \<leadsto> Let e e'"
+| ev_case2 [simp]: "lookup l cs = Some e \<Longrightarrow> Case (Inj l ts x) t cs \<leadsto> Let (Var x) e"
 | ev_case_let [simp]: "is_value e\<^sub>2 \<Longrightarrow> 
     Case (Let e\<^sub>1 e\<^sub>2) t cs \<leadsto> Let e\<^sub>1 (Case e\<^sub>2 t (map (incr\<^sub>e\<^sub>e (Suc 0)) cs))" 
-| ev_fold [simp]: "\<not> is_var e \<Longrightarrow> Fold t e \<leadsto> Let e (Fold t (Var 0))" 
 | ev_unfold1 [simp]: "e \<leadsto> e' \<Longrightarrow> Unfold t e \<leadsto> Unfold t e'"  
-| ev_unfold2 [simp]: "is_var e \<Longrightarrow> Unfold t (Fold t e) \<leadsto> e" 
+| ev_unfold2 [simp]: "Unfold t (Fold t e) \<leadsto> Var e" 
 | ev_unfold_let [simp]: "is_value e\<^sub>2 \<Longrightarrow> Unfold t (Let e\<^sub>1 e\<^sub>2) \<leadsto> Let e\<^sub>1 (Unfold t e\<^sub>2)" 
 | ev_tyapp1 [simp]: "e \<leadsto> e' \<Longrightarrow> TyApp e t \<leadsto> TyApp e' t" 
 | ev_tyapp2 [simp]: "TyApp (TyAbs k e) t \<leadsto> subst\<^sub>t\<^sub>e 0 t e" 
@@ -30,34 +27,31 @@ inductive evaluate :: "expr \<Rightarrow> expr \<Rightarrow> bool" (infix "\<lea
 
 lemma canonical_arrow [simp]: "\<Delta>,\<Gamma> \<turnstile> e : Arrow t\<^sub>1 t\<^sub>2 \<Longrightarrow> is_value e \<Longrightarrow> 
     (\<exists>e'. e = Abs t\<^sub>1 e') \<or> (\<exists>e\<^sub>1 e\<^sub>2. e = Let e\<^sub>1 e\<^sub>2 \<and> is_value e\<^sub>2)"
-  by (induction \<Gamma> e "Arrow t\<^sub>1 t\<^sub>2" rule: typecheck_typecheck_fs_typecheck_cs.inducts(1)) simp_all
+  by (induction \<Gamma> e "Arrow t\<^sub>1 t\<^sub>2" rule: typecheck_typecheck_cs.inducts(1)) simp_all
 
 lemma canonical_record [simp]: "\<Delta>,\<Gamma> \<turnstile> e : Record ts \<Longrightarrow> is_value e \<Longrightarrow> 
-    (\<exists>fs. e = Rec fs \<and> list_all is_var fs \<and> \<Delta>,\<Gamma> \<turnstile>\<^sub>f fs : ts) \<or> (\<exists>e\<^sub>1 e\<^sub>2. e = Let e\<^sub>1 e\<^sub>2 \<and> is_value e\<^sub>2)"
-  by (induction \<Gamma> e "Record ts" rule: typecheck_typecheck_fs_typecheck_cs.inducts(1)) simp_all
+    (\<exists>fs. e = Rec fs \<and> \<Delta>,\<Gamma> \<turnstile>\<^sub>x\<^sub>s fs : ts) \<or> (\<exists>e\<^sub>1 e\<^sub>2. e = Let e\<^sub>1 e\<^sub>2 \<and> is_value e\<^sub>2)"
+  by (induction \<Gamma> e "Record ts" rule: typecheck_typecheck_cs.inducts(1)) simp_all
 
 lemma canonical_variant [simp]: "\<Delta>,\<Gamma> \<turnstile> e : Variant ts \<Longrightarrow> is_value e \<Longrightarrow> 
-    (\<exists>l e'. e = Inj l ts e' \<and> is_var e' \<and> l < length ts) \<or> (\<exists>e\<^sub>1 e\<^sub>2. e = Let e\<^sub>1 e\<^sub>2 \<and> is_value e\<^sub>2)"
-  by (induction \<Gamma> e "Variant ts" rule: typecheck_typecheck_fs_typecheck_cs.inducts(1)) auto
+    (\<exists>l e'. e = Inj l ts e' \<and> l < length ts) \<or> (\<exists>e\<^sub>1 e\<^sub>2. e = Let e\<^sub>1 e\<^sub>2 \<and> is_value e\<^sub>2)"
+  by (induction \<Gamma> e "Variant ts" rule: typecheck_typecheck_cs.inducts(1)) auto
 
 lemma canonical_inductive [simp]: "\<Delta>,\<Gamma> \<turnstile> e : Inductive k t \<Longrightarrow> is_value e \<Longrightarrow> 
-    (\<exists>e'. e = Fold t e' \<and> is_var e') \<or> (\<exists>e\<^sub>1 e\<^sub>2. e = Let e\<^sub>1 e\<^sub>2 \<and> is_value e\<^sub>2)"
-  by (induction \<Gamma> e "Inductive k t" rule: typecheck_typecheck_fs_typecheck_cs.inducts(1)) auto
+    (\<exists>e'. e = Fold t e') \<or> (\<exists>e\<^sub>1 e\<^sub>2. e = Let e\<^sub>1 e\<^sub>2 \<and> is_value e\<^sub>2)"
+  by (induction \<Gamma> e "Inductive k t" rule: typecheck_typecheck_cs.inducts(1)) auto
 
 lemma canonical_forall [simp]: "\<Delta>,\<Gamma> \<turnstile> e : Forall k t \<Longrightarrow> is_value e \<Longrightarrow> 
     (\<exists>e'. e = TyAbs k e') \<or> (\<exists>e\<^sub>1 e\<^sub>2. e = Let e\<^sub>1 e\<^sub>2 \<and> is_value e\<^sub>2)"
-  by (induction \<Gamma> e "Forall k t" rule: typecheck_typecheck_fs_typecheck_cs.inducts(1)) auto
+  by (induction \<Gamma> e "Forall k t" rule: typecheck_typecheck_cs.inducts(1)) auto
 
-lemma lookup_in_tc [simp]: "\<Delta>,\<Gamma> \<turnstile>\<^sub>f fs : ts \<Longrightarrow> lookup l ts = Some t \<Longrightarrow> \<exists>e. lookup l fs = Some e"
+lemma lookup_in_tc [simp]: "\<Delta>,\<Gamma> \<turnstile>\<^sub>x\<^sub>s fs : ts \<Longrightarrow> lookup l ts = Some t \<Longrightarrow> \<exists>e. lookup l fs = Some e"
   by (induction l fs arbitrary: ts rule: lookup.induct) auto
 
 lemma progress': "\<Delta>,\<Gamma> \<turnstile> e : t \<Longrightarrow> 
   is_value e \<or> (\<exists>e'. e \<leadsto> e') \<or> (\<exists>x < length \<Gamma>. head_var e = Some x)"
-    and "\<Delta>,\<Gamma> \<turnstile>\<^sub>f fs : ts \<Longrightarrow> True"
     and "\<Delta>,\<Gamma> \<turnstile>\<^sub>c cs : ts \<rightarrow> t \<Longrightarrow> l < length ts \<Longrightarrow> \<exists>c. lookup l cs = Some c"
-  proof (induction \<Delta> \<Gamma> e t and \<Delta> \<Gamma> fs ts and \<Delta> \<Gamma> cs ts t
-         arbitrary: and and l
-         rule: typecheck_typecheck_fs_typecheck_cs.inducts)
+  proof (induction \<Delta> \<Gamma> e t and \<Delta> \<Gamma> cs ts t arbitrary: and l rule: typecheck_typecheck_cs.inducts)
   case tc_var
     thus ?case by (metis lookup_less_than head_var.simps(1))
   next case tc_app
@@ -81,17 +75,11 @@ lemma progress': "\<Delta>,\<Gamma> \<turnstile> e : t \<Longrightarrow>
               qed simp_all
           qed (metis ev_let1)
       qed simp_all
-  next case tc_rec
-    thus ?case by (metis ev_rec is_value.simps(5) split_fields)
   next case tc_proj
     thus ?case 
-      by (metis canonical_record ev_proj1 ev_proj2 ev_proj_let head_var.simps(6) lookup_in_tc)
-  next case tc_inj
-    thus ?case by (metis ev_inj is_value.simps(7))
+      by (metis canonical_record ev_proj1 ev_proj2 ev_proj_let lookup_in_tc head_var.simps(6))
   next case tc_case
     thus ?case by (metis canonical_variant ev_case1 ev_case2 ev_case_let head_var.simps(8))
-  next case tc_fold
-    thus ?case by (metis ev_fold is_value.simps(9))
   next case tc_unfold
     thus ?case by (metis canonical_inductive ev_unfold1 ev_unfold2 ev_unfold_let head_var.simps(10))
   next case tc_tyapp
@@ -105,30 +93,20 @@ lemma progress': "\<Delta>,\<Gamma> \<turnstile> e : t \<Longrightarrow>
 theorem progress: "\<Delta>,[] \<turnstile> e : t \<Longrightarrow> is_value e \<or> (\<exists>e'. e \<leadsto> e')"
   using progress' by fastforce
 
-lemma [elim]: "\<Delta>,\<Gamma> \<turnstile>\<^sub>f fs : ts \<Longrightarrow> lookup l fs = Some e \<Longrightarrow> lookup l ts = Some t \<Longrightarrow> \<Delta>,\<Gamma> \<turnstile> e : t" 
-  by (induction l fs arbitrary: ts rule: lookup.induct) auto
-
 lemma [elim]: "\<Delta>,\<Gamma> \<turnstile>\<^sub>c cs : ts \<rightarrow> t \<Longrightarrow> lookup l cs = Some e \<Longrightarrow> lookup l ts = Some t' \<Longrightarrow> 
     \<Delta>,insert_at 0 t' \<Gamma> \<turnstile> e : t" 
   by (induction l cs arbitrary: ts rule: lookup.induct) auto
 
 theorem preservation: "e \<leadsto> e' \<Longrightarrow> \<Delta>,\<Gamma> \<turnstile> e : t \<Longrightarrow> \<Delta>,\<Gamma> \<turnstile> e' : t"
   proof (induction e e' arbitrary: \<Delta> \<Gamma> t rule: evaluate.induct) 
-  case (ev_rec vs e nvs)
-    then obtain tvs tenvs where "t = Record (tvs @ tenvs) \<and> (\<Delta>,\<Gamma> \<turnstile>\<^sub>f vs : tvs) 
-      \<and> (\<Delta>,\<Gamma> \<turnstile>\<^sub>f [e] @ nvs : tenvs)" by fastforce
-    thus ?case by fastforce
-  next case (ev_inj e l ts)
-    then obtain t\<^sub>1 where T: "(\<Delta>,\<Gamma> \<turnstile> e : t\<^sub>1) \<and> lookup l ts = Some t\<^sub>1 \<and> 
-      (\<forall>tt \<in> set ts. \<Delta> \<turnstile>\<^sub>k tt : Star) \<and> t = Variant ts" by fastforce
-    have "\<Delta>,insert_at 0 t\<^sub>1 \<Gamma> \<turnstile> Var 0 : t\<^sub>1" by simp
-    with T have "\<Delta>,insert_at 0 t\<^sub>1 \<Gamma> \<turnstile> Inj l ts (Var 0) : Variant ts" by (metis tc_inj)
-    with T show ?case by (metis tc_let)
-  next case (ev_case2 e l cs e' ts t')
-    then obtain tt where "(\<Delta>,\<Gamma> \<turnstile> e : tt) \<and> lookup l ts = Some tt \<and> 
+  case (ev_proj2 l xs x)
+    hence "lookup x \<Gamma> = Some t" by fastforce
+    thus ?case by simp
+  next case (ev_case2 l cs e ts x t')
+    then obtain tt where "(lookup x \<Gamma> = Some tt) \<and> lookup l ts = Some tt \<and> 
       (\<forall>tt \<in> set ts. \<Delta> \<turnstile>\<^sub>k tt : Star) \<and> (\<Delta>,\<Gamma> \<turnstile>\<^sub>c cs : ts \<rightarrow> t') \<and> t' = t" by fastforce
-    moreover with ev_case2 have "\<Delta>,insert_at 0 tt \<Gamma> \<turnstile> e' : t" by fastforce
-    ultimately show ?case by fastforce
+    moreover with ev_case2 have "\<Delta>,insert_at 0 tt \<Gamma> \<turnstile> e : t" by fastforce
+    ultimately show ?case by (metis tc_let tc_var)
   next case (ev_tyapp2 k e t')
     then obtain tt where T: "(insert_at 0 k \<Delta>,map (incr\<^sub>t\<^sub>t 0) \<Gamma> \<turnstile> e : tt) \<and> (\<Delta> \<turnstile>\<^sub>k t' : k) \<and> 
       t = subst\<^sub>t\<^sub>t 0 t' tt" by fastforce
