01Expression/Expression.thy
@@ -7,11 +7,11 @@ datatype expr =
 | Abs type expr
 | App expr expr
 | Let expr expr
-| Rec "expr list"
+| Rec "nat list"
 | Proj expr nat
-| Inj nat "type list" expr
+| Inj nat "type list" nat
 | Case expr type "expr list"
-| Fold type expr
+| Fold type nat
 | Unfold type expr
 | TyAbs kind expr
 | TyApp expr type
@@ -22,11 +22,11 @@ primrec incr\<^sub>t\<^sub>e :: "nat \<Rightarrow> expr \<Rightarrow> expr" wher
 | "incr\<^sub>t\<^sub>e x (Abs t e) = Abs (incr\<^sub>t\<^sub>t x t) (incr\<^sub>t\<^sub>e x e)"
 | "incr\<^sub>t\<^sub>e x (App e\<^sub>1 e\<^sub>2) = App (incr\<^sub>t\<^sub>e x e\<^sub>1) (incr\<^sub>t\<^sub>e x e\<^sub>2)"
 | "incr\<^sub>t\<^sub>e x (Let e\<^sub>1 e\<^sub>2) = Let (incr\<^sub>t\<^sub>e x e\<^sub>1) (incr\<^sub>t\<^sub>e x e\<^sub>2)"
-| "incr\<^sub>t\<^sub>e x (Rec fs) = Rec (map (incr\<^sub>t\<^sub>e x) fs)"
+| "incr\<^sub>t\<^sub>e x (Rec xs) = Rec xs"
 | "incr\<^sub>t\<^sub>e x (Proj e l) = Proj (incr\<^sub>t\<^sub>e x e) l"
-| "incr\<^sub>t\<^sub>e x (Inj l ts e) = Inj l (map (incr\<^sub>t\<^sub>t x) ts) (incr\<^sub>t\<^sub>e x e)"
+| "incr\<^sub>t\<^sub>e x (Inj l ts y) = Inj l (map (incr\<^sub>t\<^sub>t x) ts) y"
 | "incr\<^sub>t\<^sub>e x (Case e t cs) = Case (incr\<^sub>t\<^sub>e x e) (incr\<^sub>t\<^sub>t x t) (map (incr\<^sub>t\<^sub>e x) cs)"
-| "incr\<^sub>t\<^sub>e x (Fold t e) = Fold (incr\<^sub>t\<^sub>t (Suc x) t) (incr\<^sub>t\<^sub>e x e)"
+| "incr\<^sub>t\<^sub>e x (Fold t y) = Fold (incr\<^sub>t\<^sub>t (Suc x) t) y"
 | "incr\<^sub>t\<^sub>e x (Unfold t e) = Unfold (incr\<^sub>t\<^sub>t (Suc x) t) (incr\<^sub>t\<^sub>e x e)"
 | "incr\<^sub>t\<^sub>e x (TyAbs k e) = TyAbs k (incr\<^sub>t\<^sub>e (Suc x) e)"
 | "incr\<^sub>t\<^sub>e x (TyApp e t) = TyApp (incr\<^sub>t\<^sub>e x e) (incr\<^sub>t\<^sub>t x t)"
@@ -37,11 +37,11 @@ primrec subst\<^sub>t\<^sub>e :: "nat \<Rightarrow> type \<Rightarrow> expr \<Ri
 | "subst\<^sub>t\<^sub>e x t' (Abs t e) = Abs (subst\<^sub>t\<^sub>t x t' t) (subst\<^sub>t\<^sub>e x t' e)"
 | "subst\<^sub>t\<^sub>e x t' (App e\<^sub>1 e\<^sub>2) = App (subst\<^sub>t\<^sub>e x t' e\<^sub>1) (subst\<^sub>t\<^sub>e x t' e\<^sub>2)"
 | "subst\<^sub>t\<^sub>e x t' (Let e\<^sub>1 e\<^sub>2) = Let (subst\<^sub>t\<^sub>e x t' e\<^sub>1) (subst\<^sub>t\<^sub>e x t' e\<^sub>2)"
-| "subst\<^sub>t\<^sub>e x t' (Rec fs) = Rec (map (subst\<^sub>t\<^sub>e x t') fs)"
+| "subst\<^sub>t\<^sub>e x t' (Rec xs) = Rec xs"
 | "subst\<^sub>t\<^sub>e x t' (Proj e l) = Proj (subst\<^sub>t\<^sub>e x t' e) l"
-| "subst\<^sub>t\<^sub>e x t' (Inj l ts e) = Inj l (map (subst\<^sub>t\<^sub>t x t') ts) (subst\<^sub>t\<^sub>e x t' e)"
+| "subst\<^sub>t\<^sub>e x t' (Inj l ts y) = Inj l (map (subst\<^sub>t\<^sub>t x t') ts) y"
 | "subst\<^sub>t\<^sub>e x t' (Case e t cs) = Case (subst\<^sub>t\<^sub>e x t' e) (subst\<^sub>t\<^sub>t x t' t) (map (subst\<^sub>t\<^sub>e x t') cs)"
-| "subst\<^sub>t\<^sub>e x t' (Fold t e) = Fold (subst\<^sub>t\<^sub>t (Suc x) (incr\<^sub>t\<^sub>t 0 t') t) (subst\<^sub>t\<^sub>e x t' e)"
+| "subst\<^sub>t\<^sub>e x t' (Fold t y) = Fold (subst\<^sub>t\<^sub>t (Suc x) (incr\<^sub>t\<^sub>t 0 t') t) y"
 | "subst\<^sub>t\<^sub>e x t' (Unfold t e) = Unfold (subst\<^sub>t\<^sub>t (Suc x) (incr\<^sub>t\<^sub>t 0 t') t) (subst\<^sub>t\<^sub>e x t' e)"
 | "subst\<^sub>t\<^sub>e x t' (TyAbs k e) = TyAbs k (subst\<^sub>t\<^sub>e (Suc x) (incr\<^sub>t\<^sub>t 0 t') e)"
 | "subst\<^sub>t\<^sub>e x t' (TyApp e t) = TyApp (subst\<^sub>t\<^sub>e x t' e) (subst\<^sub>t\<^sub>t x t' t)"
@@ -52,45 +52,41 @@ primrec incr\<^sub>e\<^sub>e :: "nat \<Rightarrow> expr \<Rightarrow> expr" wher
 | "incr\<^sub>e\<^sub>e x (Abs t e) = Abs t (incr\<^sub>e\<^sub>e (Suc x) e)"
 | "incr\<^sub>e\<^sub>e x (App e\<^sub>1 e\<^sub>2) = App (incr\<^sub>e\<^sub>e x e\<^sub>1) (incr\<^sub>e\<^sub>e x e\<^sub>2)"
 | "incr\<^sub>e\<^sub>e x (Let e\<^sub>1 e\<^sub>2) = Let (incr\<^sub>e\<^sub>e x e\<^sub>1) (incr\<^sub>e\<^sub>e (Suc x) e\<^sub>2)"
-| "incr\<^sub>e\<^sub>e x (Rec fs) = Rec (map (incr\<^sub>e\<^sub>e x) fs)"
+| "incr\<^sub>e\<^sub>e x (Rec ys) = Rec (map (\<lambda>y. if x \<le> y then Suc y else y) ys)"
 | "incr\<^sub>e\<^sub>e x (Proj e l) = Proj (incr\<^sub>e\<^sub>e x e) l"
-| "incr\<^sub>e\<^sub>e x (Inj l ts e) = Inj l ts (incr\<^sub>e\<^sub>e x e)"
+| "incr\<^sub>e\<^sub>e x (Inj l ts y) = Inj l ts (if x \<le> y then Suc y else y)"
 | "incr\<^sub>e\<^sub>e x (Case e t cs) = Case (incr\<^sub>e\<^sub>e x e) t (map (incr\<^sub>e\<^sub>e (Suc x)) cs)"
-| "incr\<^sub>e\<^sub>e x (Fold t e) = Fold t (incr\<^sub>e\<^sub>e x e)"
+| "incr\<^sub>e\<^sub>e x (Fold t y) = Fold t (if x \<le> y then Suc y else y)"
 | "incr\<^sub>e\<^sub>e x (Unfold t e) = Unfold t (incr\<^sub>e\<^sub>e x e)"
 | "incr\<^sub>e\<^sub>e x (TyAbs k e) = TyAbs k (incr\<^sub>e\<^sub>e x e)"
 | "incr\<^sub>e\<^sub>e x (TyApp e t) = TyApp (incr\<^sub>e\<^sub>e x e) t"
 | "incr\<^sub>e\<^sub>e x (TyLet t e) = TyLet t (incr\<^sub>e\<^sub>e x e)"
 
 primrec subst\<^sub>e\<^sub>e :: "nat \<Rightarrow> expr \<Rightarrow> expr \<Rightarrow> expr" where
-  "subst\<^sub>e\<^sub>e x e' (Var y) = (if x = y then e' else Var (if x < y then y - 1 else y))"
+  "subst\<^sub>e\<^sub>e x e' (Var y) = (if x = y then e' else Var y)"
 | "subst\<^sub>e\<^sub>e x e' (Abs t e) = Abs t (subst\<^sub>e\<^sub>e (Suc x) (incr\<^sub>e\<^sub>e 0 e') e)"
 | "subst\<^sub>e\<^sub>e x e' (App e\<^sub>1 e\<^sub>2) = App (subst\<^sub>e\<^sub>e x e' e\<^sub>1) (subst\<^sub>e\<^sub>e x e' e\<^sub>2)"
 | "subst\<^sub>e\<^sub>e x e' (Let e\<^sub>1 e\<^sub>2) = Let (subst\<^sub>e\<^sub>e x e' e\<^sub>1) (subst\<^sub>e\<^sub>e (Suc x) (incr\<^sub>e\<^sub>e 0 e') e\<^sub>2)"
-| "subst\<^sub>e\<^sub>e x e' (Rec fs) = Rec (map (subst\<^sub>e\<^sub>e x e') fs)"
+| "subst\<^sub>e\<^sub>e x e' (Rec ys) = Rec ys"
 | "subst\<^sub>e\<^sub>e x e' (Proj e l) = Proj (subst\<^sub>e\<^sub>e x e' e) l"
-| "subst\<^sub>e\<^sub>e x e' (Inj l ts e) = Inj l ts (subst\<^sub>e\<^sub>e x e' e)"
+| "subst\<^sub>e\<^sub>e x e' (Inj l ts y) = Inj l ts y"
 | "subst\<^sub>e\<^sub>e x e' (Case e t cs) = Case (subst\<^sub>e\<^sub>e x e' e) t (map (subst\<^sub>e\<^sub>e (Suc x) (incr\<^sub>e\<^sub>e 0 e')) cs)"
-| "subst\<^sub>e\<^sub>e x e' (Fold t e) = Fold t (subst\<^sub>e\<^sub>e x e' e)"
+| "subst\<^sub>e\<^sub>e x e' (Fold t y) = Fold t y"
 | "subst\<^sub>e\<^sub>e x e' (Unfold t e) = Unfold t (subst\<^sub>e\<^sub>e x e' e)"
 | "subst\<^sub>e\<^sub>e x e' (TyAbs k e) = TyAbs k (subst\<^sub>e\<^sub>e x (incr\<^sub>t\<^sub>e 0 e') e)"
 | "subst\<^sub>e\<^sub>e x e' (TyApp e t) = TyApp (subst\<^sub>e\<^sub>e x e' e) t"
 | "subst\<^sub>e\<^sub>e x e' (TyLet t e) = TyLet t (subst\<^sub>e\<^sub>e x (incr\<^sub>t\<^sub>e 0 e') e)"
-
-fun is_var :: "expr \<Rightarrow> bool" where
-  "is_var (Var x) = True"
-| "is_var _ = False"
 
 primrec is_value :: "expr \<Rightarrow> bool" where
   "is_value (Var x) = False"
 | "is_value (Abs t e) = True"
 | "is_value (App e\<^sub>1 e\<^sub>2) = False"
 | "is_value (Let e\<^sub>1 e\<^sub>2) = is_value e\<^sub>2"
-| "is_value (Rec fs) = list_all is_var fs"
+| "is_value (Rec fs) = True"
 | "is_value (Proj e l) = False"
-| "is_value (Inj l ts e) = is_var e"
+| "is_value (Inj l ts e) = True"
 | "is_value (Case e t cs) = False"
-| "is_value (Fold t e) = is_var e"
+| "is_value (Fold t e) = True"
 | "is_value (Unfold t e) = False"
 | "is_value (TyAbs k e) = True"
 | "is_value (TyApp e t) = False"
@@ -120,21 +116,6 @@ lemma [simp]: "size (subst\<^sub>t\<^sub>e x t e) = size e"
     thus ?case by (induction es) simp_all
   next case (Case e t cs)
     thus ?case by (induction cs) simp_all
-  qed simp_all
-
-lemma split_fields [simp]: "\<not> list_all is_var fs \<Longrightarrow> 
-    \<exists>vs e nvs. fs = vs @ [e] @ nvs \<and> list_all is_var vs \<and> \<not> is_var e"
-  proof (induction fs)
-  case (Cons f fs)
-    thus ?case
-      proof (cases "is_var f")
-      case True
-        with Cons obtain vs e nvs where "fs = vs @ [e] @ nvs \<and> list_all is_var vs \<and> \<not> is_var e" 
-          by fastforce
-        with True have "f # fs = (f # vs) @ [e] @ nvs \<and> list_all is_var (f # vs) \<and> \<not> is_var e" 
-          by simp
-        thus ?thesis by blast
-      qed fastforce+
   qed simp_all
 
 end
