01Expression/Determinism.thy
@@ -8,20 +8,8 @@ lemma [elim]: "head_var e = Some x \<Longrightarrow> is_value e \<Longrightarrow
 lemma [elim]: "e \<leadsto> e' \<Longrightarrow> is_value e \<Longrightarrow> False"
   by (induction e e' rule: evaluate.induct) auto
 
-lemma [elim]: "e \<leadsto> e' \<Longrightarrow> is_var e \<Longrightarrow> False"
-  by (induction e e' rule: evaluate.induct) simp_all
-
 lemma [elim]: "e \<leadsto> e' \<Longrightarrow> head_var e = Some x \<Longrightarrow> False"
   by (induction e e' arbitrary: x rule: evaluate.induct) (auto split: option.splits nat.splits)
-
-lemma [elim]: "list_all is_var vs \<Longrightarrow> list_all is_var vs' \<Longrightarrow> \<not> is_var e \<Longrightarrow> \<not> is_var e' \<Longrightarrow>
-    vs @ [e] @ nvs = vs' @ [e'] @ nvs' \<Longrightarrow> vs = vs'"
-  proof (induction vs arbitrary: vs')
-  case Nil
-    thus ?case by (induction vs') simp_all
-  next case (Cons v vs)
-    thus ?case by (induction vs') simp_all
-  qed
 
 theorem determinism [elim]: "e \<leadsto> e' \<Longrightarrow> e \<leadsto> e'' \<Longrightarrow> e' = e''"
   proof (induction e e' arbitrary: e'' rule: evaluate.induct)
@@ -74,13 +62,6 @@ theorem determinism [elim]: "e \<leadsto> e' \<Longrightarrow> e \<leadsto> e'' 
         hence False by auto
         thus ?case by simp
       qed simp_all
-  next case (ev_rec vs e nvs)
-    with ev_rec(3) show ?case
-      proof (induction "Rec (vs @ [e] @ nvs)" e'' rule: evaluate.induct)
-      case (ev_rec vs' e\<^sub>2 nvs')
-        hence "vs' = vs" by auto
-        with ev_rec show ?case by simp
-      qed
   next case (ev_proj1 e e' l)
     with ev_proj1(3) show ?case
       proof (induction "Proj e l" e'' rule: evaluate.induct)
@@ -91,8 +72,8 @@ theorem determinism [elim]: "e \<leadsto> e' \<Longrightarrow> e \<leadsto> e'' 
         hence False by auto
         thus ?case by simp
       qed simp_all
-  next case (ev_proj2 fs l e)
-    with ev_proj2(3) show ?case
+  next case (ev_proj2 l fs e)
+    with ev_proj2(2) show ?case
       proof (induction "Proj (Rec fs) l" e'' rule: evaluate.induct)
       case ev_proj1
         hence False by auto
@@ -105,8 +86,6 @@ theorem determinism [elim]: "e \<leadsto> e' \<Longrightarrow> e \<leadsto> e'' 
         hence False by auto
         thus ?case by simp
       qed simp_all
-  next case (ev_inj e l ts)
-    with ev_inj(2) show ?case by (induction "Inj l ts e" e'' rule: evaluate.induct) simp_all
   next case (ev_case1 e e' t cs)
     with ev_case1(3) show ?case
       proof (induction "Case e t cs" e'' rule: evaluate.induct)
@@ -117,8 +96,8 @@ theorem determinism [elim]: "e \<leadsto> e' \<Longrightarrow> e \<leadsto> e'' 
         hence False by auto
         thus ?case by simp
       qed simp_all
-  next case (ev_case2 e l cs e' ts t)
-    with ev_case2(3) show ?case
+  next case (ev_case2 l cs e' ts e t)
+    with ev_case2(2) show ?case
       proof (induction "Case (Inj l ts e) t cs" e'' rule: evaluate.induct)
       case ev_case1
         hence False by auto
@@ -131,8 +110,6 @@ theorem determinism [elim]: "e \<leadsto> e' \<Longrightarrow> e \<leadsto> e'' 
         hence False by auto
         thus ?case by simp
       qed simp_all
-  next case (ev_fold e t)
-    with ev_fold(2) show ?case by (induction "Fold t e" e'' rule: evaluate.induct) simp_all
   next case (ev_unfold1 e e' t)
     with ev_unfold1(3) show ?case
       proof (induction "Unfold t e" e'' rule: evaluate.induct)
@@ -143,8 +120,8 @@ theorem determinism [elim]: "e \<leadsto> e' \<Longrightarrow> e \<leadsto> e'' 
         hence False by auto
         thus ?case by simp
       qed simp_all
-  next case (ev_unfold2 e t)
-    with ev_unfold2(2) show ?case
+  next case (ev_unfold2 t e)
+    thus ?case
       proof (induction "Unfold t (Fold t e)" e'' rule: evaluate.induct)
       case ev_unfold1
         hence False by auto
@@ -175,12 +152,8 @@ theorem determinism [elim]: "e \<leadsto> e' \<Longrightarrow> e \<leadsto> e'' 
         thus ?case by simp
       qed simp_all
   next case (ev_tyapp_let e\<^sub>2 e\<^sub>1 t)
-    with ev_tyapp_let(2) show ?case
-      proof (induction "TyApp (Let e\<^sub>1 e\<^sub>2) t" e'' rule: evaluate.induct)
-      case ev_tyapp1
-        hence False by auto
-        thus ?case by simp
-      qed simp_all
+    with ev_tyapp_let(2) show ?case 
+      by (induction "TyApp (Let e\<^sub>1 e\<^sub>2) t" e'' rule: evaluate.induct) auto
   next case (ev_tylet t e)
     thus ?case by (induction "TyLet t e" e'' rule: evaluate.induct) simp_all
   qed
